src/Day12.v
@@ -1,0 +1,113 @@
+From Coq Require Export String List NArith Ascii.
+From Coq Require Import Lia Sorting Orders OrdersEx OrdersAlt FMapAVL Program.Wf.
+
+Import IfNotations.
+Export StringSyntax ListNotations.
+
+#[global] Open Scope char_scope.
+#[global] Open Scope nat_scope.
+#[global] Open Scope N_scope.
+
+Inductive status : Set :=
+| Operational | Damaged | Unknown.
+Inductive spring_rec : Type :=
+  mkrec : list status -> list N -> spring_rec.
+
+Definition status_of_ascii (c : ascii) : status :=
+  match c with
+  | "#" => Damaged
+  | "." => Operational
+  | _ => Unknown
+  end.
+Definition statuses_of_string (s : string) : list status :=
+  List.map status_of_ascii (list_ascii_of_string s).
+
+Fixpoint head_matches_ (i : nat) (s : list status) (g : nat) : option nat :=
+  match (g, s) with
+  | (S g', (Damaged | Unknown) :: s') => head_matches_ (S i) s' g'
+  | (S _, (Operational :: _ | [])) => None
+  | (O, (Operational | Unknown) :: _) => Some (S i)
+  | (O, []) => Some i
+  | (O, Damaged :: _) => None
+  end.
+Definition head_matches := head_matches_ O.
+Definition get_valid_steps (s : list status) (gs : list N) : list (option nat) :=
+  List.map (fun g => head_matches s (N.to_nat g)) gs.
+
+Fixpoint count_valid_groupings_ (prev_not_damaged : N) (s : list status) (gs : list N) : list (list N) :=
+  match s with
+  | [] => [List.map (fun _ => 0) gs ++ [1]]
+  | fc::s' =>
+      let not_damaged := if fc is Damaged then 0 else 1 in
+      let dp := count_valid_groupings_ not_damaged s' gs in
+      let next_col := List.hd [] dp in
+      let tl_can_be_empty :=
+        if nth (List.length gs) next_col 0 =? 1 (* next col can be empty *)
+        then not_damaged (* can still be empty *)
+        else 0 in
+      let valid_steps :=
+        (*if prev_not_damaged =? 1
+        then*) get_valid_steps s gs
+        (*else List.map (fun _ => None) gs*) in
+      let step_all :=
+        List.fold_left
+          (fun '(acc, i) is_valid =>
+             let next_cnt :=
+               if not_damaged =? 1
+               then nth i next_col 0
+               else 0 (* if it is damaged we cannot just ignore it *) in
+             let skip_cnt :=
+               match is_valid with
+               | None => 0
+               | Some len =>
+                   let skip_col := nth (pred len) dp [] in
+                   nth (S i) skip_col 0
+               end in
+             (next_cnt + skip_cnt :: acc, S i))
+          valid_steps
+          ([], O)
+      in
+      List.rev (tl_can_be_empty :: fst step_all) :: dp
+  end.
+Definition count_valid_groupings (r : spring_rec) :=
+  let '(mkrec s gs) := r in
+  let all_groupings := count_valid_groupings_ 1 s gs in
+  hd 0 (hd [] all_groupings).
+
+Definition unfold_rec (r : spring_rec) : spring_rec :=
+  let '(mkrec s gs) := r in
+  let s' := List.tl (flat_map id (List.repeat (Unknown :: s) 5)) in
+  let gs' := flat_map id (List.repeat gs 5) in
+  mkrec s' gs'.
+
+Definition part (f : spring_rec -> spring_rec) (inp : list spring_rec) :=
+  let mapped := List.map f inp in
+  let groupings := List.map count_valid_groupings mapped in
+  List.fold_left N.add groupings 0.
+
+Definition main (inp : list spring_rec) :=
+  (part id inp, part unfold_rec inp).
+
+Declare Custom Entry record.
+Declare Custom Entry groups.
+Notation "'input' record .. records" :=
+  (cons record .. (cons records nil) ..)
+    (at level 200, record custom record at level 2, only parsing).
+Notation "conds groups" :=
+  (mkrec (statuses_of_string conds) groups)
+    (in custom record at level 2, conds constr at level 1, groups custom groups at level 1).
+Notation "g ',' .. ',' gs" :=
+  (cons g .. (cons gs nil) ..)
+    (in custom groups at level 1, g constr at level 1).
+
+Definition example := input
+"???.###" 1,1,3
+".??..??...?##." 1,1,3
+"?#?#?#?#?#?#?#?" 1,3,1,6
+"????.#...#..." 4,1,1
+"????.######..#####." 1,6,5
+"?###????????" 3,2,1
+.
+
+Example sample: main example = (21, 525152).
+Proof. reflexivity. Qed.
