scripts/gen_coqproject.sh
@@ -1,0 +1,10 @@
+#!/usr/bin/env sh
+
+DIR="$(readlink -f "$(dirname "$0")"/..)"
+cd "$DIR" || exit 1
+
+SRC="$(find src -name '*.v' | sort)"
+DAYS_IN="$(printf "%s\n" $SRC | grep Day | sed -e s/Day/DayIn/g -e s/src/processed/g)"
+
+cat _CoqProject.in
+printf "%s\n" $SRC $DAYS_IN
